src/Pipit.System.Ind.fst
@@ -1,3 +1,43 @@
 module Pipit.System.Ind
 
 open Pipit.System.Base
+
+module C = Pipit.Context
+
+let base_case (#input #state: Type) (t: stepfun input state prop): prop =
+  forall (i: input) (s': state) (r: prop).
+    t i None s' r ==> r
+
+let step_case (#input #state: Type) (t: stepfun input state prop): prop =
+  forall (i0 i1: input) (s0: option state) (s1 s2: state) (r0 r1: prop).
+    t i0 s0 s1 r0 ==> r0 ==>
+    t i1 (Some s1) s2 r1 ==> r1
+
+let induct1 (#input #state: Type)
+  (t: stepfun input state prop): prop =
+    base_case t /\ step_case t
+
+let rec prop_for_all (l: list prop): prop =
+ match l with
+ | [] -> True
+ | p :: ps -> p /\ prop_for_all ps
+
+let rec induct1_sound (#len: nat { len > 0 }) (#input #state: Type)
+  (t: stepfun input state prop)
+  (inputs: C.vector input len)
+  (props: C.vector prop len)
+  (s': option state):
+    Lemma
+        (requires system_stepn' t inputs props s' /\ induct1 t)
+        (ensures prop_for_all props) =
+ match inputs, props with
+ | [i], [p] ->
+   ()
+ | i1 :: i0 :: is, p1 :: p0 :: ps ->
+   assert (len >= 2);
+   eliminate exists (s0: option state) (s1: state).
+     system_stepn' #(len - 2) t is ps s0 /\
+     t i0 s0 s1 p0
+   returns prop_for_all props
+   with h.
+     induct1_sound #(len - 1) t (i0 :: is) (p0 :: ps) (Some s1)
